cava/Cava/Monad/CavaMonad.v
@@ -17,5 +17,6 @@
 Require Export Cava.Monad.CavaClass.
 Require Export Cava.Signal.
 Require Export Cava.Monad.CombinationalMonad.
+Require Export Cava.Monad.Sequential.
 Require Export Cava.Monad.Combinators.
 Require Export Cava.Monad.NetlistGeneration.
