cava/Cava/Monad/CombinationalMonad.v
@@ -167,6 +167,12 @@ Definition greaterThanOrEqualBool {m n : nat}
 Definition bufBool (i : bool) : ident bool :=
   ret i.
 
+Definition loopBool (A B C : SignalType)
+                    (f : combType A * combType C -> ident (combType B * combType C))
+                    (a : combType A) : ident (combType B) :=
+  '(b, _) <- f (a, @defaultCombValue C) ;;
+  ret b.
+
 (******************************************************************************)
 (* Instantiate the Cava class for a boolean combinational logic               *)
 (* interpretation.                                                            *)
@@ -203,6 +209,9 @@ Definition bufBool (i : bool) : ident bool :=
     greaterThanOrEqual m n := @greaterThanOrEqualBool m n;
     instantiate _ circuit := circuit;
     blackBox intf _ := ret (tupleInterfaceDefault (map port_type (circuitOutputs intf)));
+    (* Members that ought to be in a Sequential class. Dummy definitions. *)
+    delay _ i := ret i;
+    loop a b c := @loopBool a b c;
 }.
 
 (******************************************************************************)
